{
 "cells": [
  {
   "attachments": {},
   "cell_type": "markdown",
   "metadata": {},
   "source": [
    "## Mason Wheeler\n",
    "### 5/3/2023\n",
    "### EE 242, Assignment 4"
   ]
  },
  {
   "attachments": {},
   "cell_type": "markdown",
   "metadata": {},
   "source": [
    "## 1.\n",
    "Computing the convolution 𝑥(𝑡) ∗ ℎ(𝑡):\n",
    "\n",
    "1. 𝑥(𝑡):\n",
    "    $$\\mathbf{x}(t) = \n",
    "    \\begin{cases} \n",
    "        1, & -1 \\le t < 0 \\\\\n",
    "        1 - t, & 0 \\le t \\le 1 \\\\\n",
    "        0, & \\text{otherwise}\n",
    "    \\end{cases}$$\n",
    "\n",
    "2. ℎ(𝑡):\n",
    "    $$\\mathbf{h}(t) = \n",
    "    \\begin{cases} \n",
    "        1, & -2 \\le t \\le 2 \\\\\n",
    "        0, & \\text{otherwise}\n",
    "    \\end{cases}$$\n",
    "\n",
    "Convolution formula:\n",
    "$$(\\mathbf{x} * \\mathbf{h})(\\tau) = \\int_{-\\infty}^{\\infty} \\mathbf{x}(t) \\mathbf{h}(\\tau - t) dt$$\n",
    "\n",
    "Considering the different cases for the convolution:\n",
    "\n",
    "- For $\\tau < -3$, the functions do not overlap, so the convolution is 0.\n",
    "\n",
    "- For $-3 \\le \\tau < -2$:\n",
    "  $$(\\mathbf{x} * \\mathbf{h})(\\tau) = \\int_{\\tau+2}^{0} \\mathbf{x}(t) \\mathbf{h}(\\tau - t) dt$$\n",
    "  $$(\\mathbf{x} * \\mathbf{h})(\\tau) = \\int_{\\tau+2}^{0} dt$$\n",
    "  $$(\\mathbf{x} * \\mathbf{h})(\\tau) = \\tau + 2$$\n",
    "\n",
    "- For $-2 \\le \\tau < -1$:\n",
    "  $$(\\mathbf{x} * \\mathbf{h})(\\tau) = \\int_{\\tau+2}^{1} \\mathbf{x}(t) \\mathbf{h}(\\tau - t) dt$$\n",
    "  $$(\\mathbf{x} * \\mathbf{h})(\\tau) = \\int_{\\tau+2}^{1} dt$$\n",
    "  $$(\\mathbf{x} * \\mathbf{h})(\\tau) = 3 + \\tau$$\n",
    "\n",
    "- For $-1 \\le \\tau < 0$:\n",
    "  $$(\\mathbf{x} * \\mathbf{h})(\\tau) = \\int_{0}^{\\tau+2} \\mathbf{x}(t) \\mathbf{h}(\\tau - t) dt$$\n",
    "  $$(\\mathbf{x} * \\mathbf{h})(\\tau) = \\int_{0}^{\\tau+2} dt$$\n",
    "  $$(\\mathbf{x} * \\mathbf{h})(\\tau) = \\tau + 2$$\n",
    "\n",
    "- For $0 \\le \\tau < 1$:\n",
    "  $$(\\mathbf{x} * \\mathbf{h})(\\tau) = \\int_{\\tau-2}^{1} (1 - t) \\mathbf{h}(\\tau - t) dt$$\n",
    "  $$(\\mathbf{x} * \\mathbf{h})(\\tau) = \\int_{\\tau-2}^{1} (1 - t) dt$$\n",
    "  $$(\\mathbf{x} * \\mathbf{h})(\\tau) = \\frac{1}{2}(3 - \\tau)(1 + \\tau)\n"
   ]
  },
  {
   "attachments": {},
   "cell_type": "markdown",
   "metadata": {},
   "source": [
    "## 2.\n",
    "We can analyze the given impulse responses:\n",
    "\n",
    "**a) $h[n] = (2)^n * u[n - 2] u[n + 2]$**\n",
    "\n",
    "(i) Causal:\n",
    "Since the impulse response is 0 for n < 2 and non-zero for n ≥ 2, the system is causal.\n",
    "\n",
    "(ii) Stable:\n",
    "The impulse response has an exponential growth term (2)^n, which makes the system unstable.\n",
    "\n",
    "**b) $h[n] = (n * (0.5)^n) * u[n - 1]$**\n",
    "\n",
    "(i) Causal:\n",
    "Since the impulse response is 0 for n < 1 and non-zero for n ≥ 1, the system is causal.\n",
    "\n",
    "(ii) Stable:\n",
    "The impulse response has an exponential decay term (0.5)^n, which makes the system stable.\n",
    "\n",
    "**c) $h(t) = sin(t + 1) u(t - 1) + cos(t - 1) u(-t + 1)$**\n",
    "\n",
    "(i) Causal:\n",
    "Since the impulse response is 0 for t < 1, the system is causal.\n",
    "\n",
    "(ii) Stable:\n",
    "Both sine and cosine functions are bounded between -1 and 1, so the system is stable.\n",
    "\n",
    "**d) $h(t) = e^{-5|t|}$**\n",
    "\n",
    "(i) Causal:\n",
    "The impulse response is non-zero for all t, so the system is non-causal.\n",
    "\n",
    "(ii) Stable:\n",
    "The impulse response has an exponential decay term e^{-5|t|}, which makes the system stable.\n"
   ]
  },
  {
   "attachments": {},
   "cell_type": "markdown",
   "metadata": {},
   "source": [
    "## 3.\n",
    "We can analyze the given impulse responses and determine their stability by converting them to polar form:\n",
    "\n",
    "**a) $h[n] = \\left(\\frac{1}{2}+j\\frac{2}{3}\\right)^n u[n]$**\n",
    "\n",
    "In polar form:\n",
    "$h[n] = \\rho^n e^{j\\theta n} u[n]$\n",
    "\n",
    "where $\\rho = \\sqrt{\\left(\\frac{1}{2}\\right)^2 + \\left(\\frac{2}{3}\\right)^2} = \\frac{\\sqrt{13}}{6}$ and $\\theta = \\tan^{-1}\\left(\\frac{2}{3}\\right)$\n",
    "\n",
    "Since $\\rho < 1$ and $u[n]$ is causal, the system is **stable**.\n",
    "\n",
    "**b) $h[n] = \\left(\\frac{1}{2}+j\\frac{2}{3}\\right)^n u[-n]$**\n",
    "\n",
    "In polar form:\n",
    "$h[n] = \\rho^n e^{j\\theta n} u[-n]$\n",
    "\n",
    "where $\\rho$ and $\\theta$ are the same as in part (a).\n",
    "\n",
    "Since $\\rho < 1$ and $u[-n]$ is non-causal, the system is **unstable**.\n",
    "\n",
    "**c) $h(t) = e^{\\left(\\frac{1}{2}-j\\frac{2}{3}\\right)t}u(t)$**\n",
    "\n",
    "In polar form:\n",
    "$h(t) = e^{(\\frac{1}{2}t)} e^{-j\\frac{2}{3}t} u(t)$\n",
    "\n",
    "Since the exponential term $e^{\\frac{1}{2}t}$ has a positive exponent and $u(t)$ is causal, the system is **unstable**.\n",
    "\n",
    "**d) $h(t) = e^{\\left(\\frac{1}{2}-j\\frac{2}{3}\\right)t}u(-t)$**\n",
    "\n",
    "In polar form:\n",
    "$h(t) = e^{(\\frac{1}{2}t)} e^{-j\\frac{2}{3}t} u(-t)$\n",
    "\n",
    "Since the exponential term $e^{\\frac{1}{2}t}$ has a positive exponent and $u(-t)$ is non-causal, the system is **unstable**.\n"
   ]
  }
 ],
 "metadata": {
  "kernelspec": {
   "display_name": "base",
   "language": "python",
   "name": "python3"
  },
  "language_info": {
   "codemirror_mode": {
    "name": "ipython",
    "version": 3
   },
   "file_extension": ".py",
   "mimetype": "text/x-python",
   "name": "python",
   "nbconvert_exporter": "python",
   "pygments_lexer": "ipython3",
   "version": "3.9.12"
  },
  "orig_nbformat": 4
 },
 "nbformat": 4,
 "nbformat_minor": 2
}
